Implemented compression for Argon2i Indexing still unimplemented

specs/Spec.Argon2i.fst
@@ -91,6 +91,98 @@ let h' t_len x_len x =
     in
     update_slice output (r * 32) ((r*32)+64) vlast
 
+let low_bits x = to_u64 (to_u32 #U64 x)
+
+type idx = idx:size_nat{idx <= 15}
+
+let g (a:uint64) (b:uint64) (c:uint64) (d:uint64) =
+  let a = a +. b +. (u64 2) *. (low_bits a) *. (low_bits b) in
+  let d = (d ^. a) >>>. (u32 32) in
+  let c = c +. d +. (u64 2) *. (low_bits c) *. (low_bits d) in
+  let b = (b ^. c) >>>. (u32 24) in
+  let a = a +. b +. (u64 2) *. (low_bits a) *. (low_bits b) in
+  let d = (d ^. a) >>>. (u32 16) in
+  let c = c +. d +. (u64 2) *. (low_bits c) *. (low_bits d) in
+  let b = (b ^. c) >>>. (u32 63) in
+  (a,b,c,d)
+
+let permutation_matrix_index_to_offset (i:idx) : Tot size_nat =
+   if i % 2 = 0 then
+     8*((i/2)+1)
+   else
+     8*(i/2)
+
+let apply_g (v:lbytes 128) (i1:idx) (i2:idx) (i3:idx) (i4:idx) : Tot (lbytes 128) =
+  let o1 = permutation_matrix_index_to_offset i1 in
+  let o2 = permutation_matrix_index_to_offset i2 in
+  let o3 = permutation_matrix_index_to_offset i3 in
+  let o4 = permutation_matrix_index_to_offset i4 in
+  let a = uint_from_bytes_be #U64 (sub v o1 8) in
+  let b = uint_from_bytes_be #U64 (sub v o2 8) in
+  let c = uint_from_bytes_be #U64 (sub v o3 8) in
+  let d = uint_from_bytes_be #U64 (sub v o4 8) in
+  let (a,b,c,d) = g a b c d in
+  let v = update_slice v o1 (o1 + 8) (uint_to_bytes_be a) in
+  let v = update_slice v o2 (o2 + 8) (uint_to_bytes_be b) in
+  let v = update_slice v o3 (o3 + 8) (uint_to_bytes_be c) in
+  let v = update_slice v o4 (o4 + 8) (uint_to_bytes_be d) in
+  v
+
+val argon_permute : input: lbytes 128 -> Tot (lbytes 128)
+
+let argon_permute input =
+  let v : lbytes 128 = apply_g input 0 4 8 12 in
+  let v : lbytes 128 = apply_g v 1 5 9  13 in
+  let v : lbytes 128 = apply_g v 2 6 10 14 in
+  let v : lbytes 128 = apply_g v 3 7 11 15 in
+  let v : lbytes 128 = apply_g v 0 5 10 15 in
+  let v : lbytes 128 = apply_g v 1 6 11 12 in
+  let v : lbytes 128 = apply_g v 2 7 8  13 in
+  let v : lbytes 128 = apply_g v 3 4 9  14 in
+  v
+
+
+
+let xor_matrices (x:lbytes 1024) (y:lbytes 1024) : Tot (lbytes 1024) =
+  let r = create 1024 (u8 0) in
+  repeati (1024 / 8) (fun i r ->
+    update_slice r (8*i) (8*(i+1)) (uint_to_bytes_be (
+      (uint_from_bytes_be #U64 (sub x (8*i) 8)) ^. (uint_from_bytes_be #U64 (sub y (8*i) 8))
+    ))
+  ) r
+
+let extract_column_from_matrix (r: lbytes 1024) (j:size_nat{j < 8}) : Tot (lbytes 128) =
+  let output = create 128 (u8 0) in
+  let output = repeati 8 (fun i output ->
+    update_slice output (i*16) ((i+1)*16) (sub r (i*128 + j*16) 16)
+  ) output
+  in
+  output
+
+let update_column_to_matrix (col:lbytes 128) (r:lbytes 1024) (j:size_nat{j < 8}) : Tot (lbytes 1024) =
+  repeati 8 (fun i r ->
+    update_slice r (i*128 + j*16) (i*128 + (j+1)*16) (sub col (i*16) 16)
+  ) r
+
+let argon_compress (x:lbytes 1024) (y:lbytes 1024) : Tot (lbytes 1024) =
+  let r = create 1024 (u8 0) in
+  let r = xor_matrices x y in
+  (* permute rows *)
+  let q = repeati (1024 / 128) (fun i r ->
+    let row = sub r (128*i) 128 in
+    let row = argon_permute row in
+    update_slice r (128*i) (128*(i+1)) row
+  ) r in
+  (* permute columns *)
+  let z = repeati (1024 / 128) (fun j q ->
+    let col = extract_column_from_matrix q j in
+    let col = argon_permute col in
+    update_column_to_matrix col q j
+  ) q in
+  xor_matrices z r
+
+
+
 let fill_block (d_len: size_nat{d_len <= size_of_block}) (d: lbytes d_len) : Tot (lbytes size_of_block) =
   let output = create size_of_block (u8 0) in
   update_slice output 0 d_len d
@@ -138,15 +230,15 @@ let step4 t_len lanes columns mem h0 =
 val step5 : t_len:size_nat{1 <= t_len /\ t_len <= size_of_block - 64} -> lanes:size_nat{lanes >= 1 /\ lanes <= pow2 24 - 1} -> columns:size_nat{4 <= columns /\ lanes * columns * size_of_block <= max_size_t} -> mem: lbytes (lanes * columns * size_of_block) -> Tot (lbytes (lanes * columns * size_of_block))
 
 let step5 t_len lanes columns mem =
-  repeati lanes (fun i mem ->
-    repeati (columns-1) (fun j mem ->
+  repeati lanes (fun i (mem: lbytes (lanes*columns*size_of_block)) ->
+    repeati (columns-1) (fun j (mem:lbytes (lanes*columns*size_of_block)) ->
       let j = j + 1 in
       let offset = block_offset lanes columns i j in
       let first_block = sub mem (block_offset lanes columns i (j-1)) size_of_block in
-      let second_block = sub mem (block_offset lanes colmuns i j (*TODO*)) size_of_block in
-      let slice = create size_of_block (u8 0) (*TODO*)  in
+      let second_block = sub mem (block_offset lanes columns i j (*TODO*)) size_of_block in
+      let slice = argon_compress first_block second_block  in
       update_slice mem offset (offset+ size_of_block) slice
-    )
+    ) mem
   ) mem
 
 
